theories/L7/L6_to_Clight_correct.v
@@ -307,7 +307,7 @@ Proof.
   eapply t_trans; eauto.
 Qed.
 
-Theorem dsubterm_case:
+Theorem dsubterm_case_cons:
   forall v l e',
     dsubterm_e e' (Ecase v l) -> 
   forall a, dsubterm_e e' (Ecase v (a:: l)).
@@ -325,7 +325,7 @@ forall v l e',
 Proof.  
   intros. remember (Ecase v l) as y. revert dependent v. revert l. induction H.
   - intros. subst. constructor.
-    eapply dsubterm_case; eauto.
+    eapply dsubterm_case_cons; eauto.
   - intros. apply IHclos_trans2 in Heqy.
     eapply t_trans. apply H. eauto.
 Qed.
@@ -661,7 +661,7 @@ Ltac archi_red :=
    Ltac int_max_unsigned:=  
      unfold Int64.max_unsigned in *;
      unfold Int.max_unsigned in *.
-     
+
 
    
   (* Any valid mem is disjoint  the global_env *)
@@ -670,20 +670,20 @@ Ltac archi_red :=
  Inductive header_of_rep: cRep -> Z -> Prop :=
  | header_enum: forall t, header_of_rep (enum t) (Z.of_N ((N.shiftl t 1) + 1))
  | header_boxed: forall t a, header_of_rep (boxed t a) (Z.of_N ((N.shiftl a 10) + t)).
-  
+
  Function var_or_funvar_f (x:positive):expr :=
    match Genv.find_symbol (Genv.globalenv p) x with
-   | Some _ => funVar x
+   | Some _ =>  makeVar threadInfIdent x fenv
    | None => var x
    end.
-
+ 
  (* The full the domain of map is exactly the symbols of globalenv *)
  Definition find_symbol_domain {A} (map:M.t A):=
-   forall (x:positive) V1 (b:block), M.get x map = Some V1 <-> Genv.find_symbol (Genv.globalenv p) x = Some b.
+   forall (x:positive), (exists V1, M.get x map = Some V1) <-> (exists b, Genv.find_symbol (Genv.globalenv p) x = Some b).
  
-                                         
+(* CHANGE THIS *)                                    
 Inductive repr_asgn_fun': list positive -> list N -> statement -> Prop :=
-| repr_asgn_nil: forall y i,  repr_asgn_fun' [y] [i] (args[ Z.of_N i ] :::= (var_or_funvar_f y))
+| repr_asgn_nil: repr_asgn_fun' [] [] Sskip
 | repr_asgn_cons: forall y ys i inf s, repr_asgn_fun' ys inf s ->
                  repr_asgn_fun' (y::ys) (i::inf) (s; args[ Z.of_N i ] :::= (var_or_funvar_f y)).
 
@@ -772,7 +772,7 @@ Definition Forall_statements_in_seq {A}: (BinNums.Z  -> A -> statement -> Prop) 
 Inductive var_or_funvar : positive -> expr -> Prop :=
 | F_VoF : forall x b,
     Genv.find_symbol (Genv.globalenv p) x = Some b ->
-                var_or_funvar x (funVar x)
+                var_or_funvar x (makeVar threadInfIdent x fenv)
 | V_VoF : forall x,
     Genv.find_symbol (Genv.globalenv p) x = None ->
        var_or_funvar x (var x).
@@ -785,8 +785,6 @@ Proof.
   inv H;  rewrite H0; auto. 
   destruct ( Genv.find_symbol (Genv.globalenv p) x) eqn:Hx; subst; econstructor; eauto.
 Qed.
-
-
   
 Fixpoint Vint_or_Vptr (v:Values.val): bool :=
   match v with
@@ -795,7 +793,6 @@ Fixpoint Vint_or_Vptr (v:Values.val): bool :=
   | Vptr _ _ => true
   | _ => false
   end.
-
 
 Inductive get_var_or_funvar (lenv: temp_env): positive -> Values.val -> Prop :=
 |F_gVoF:
@@ -1019,7 +1016,7 @@ Proof.
   induction vs1; intros.
   - simpl in H1; subst. simpl in H0. inv H. auto.
   -   simpl in H1. inv H.
-      rewrite <- app_assoc. eapply IHvs1. apply H6. Focus 2. reflexivity.
+      rewrite <- app_assoc. eapply IHvs1. apply H6. 2: reflexivity.
       simpl.
       simpl length in H0. rewrite Nat2Z.inj_succ in H0.
       econstructor; eauto.
@@ -1530,16 +1527,16 @@ Proof.
     rewrite IHc.
     rewrite pos_iter_xO.
     rewrite pos_iter_xO.
-    Focus 2. intros. apply H.
+    2:{ intros. apply H.
     rewrite Pos2Z.inj_xO.
     assert (0 < Z.pos c)%Z by apply Pos2Z.is_pos.
-    omega.     
+    omega. }
     rewrite IHc. reflexivity.
     intros.
     assert (Hrw := Z.shiftr_spec).
     specialize (Hrw a (Z.pos c)). unfold Z.shiftr in Hrw.
     simpl in Hrw.  rewrite Hrw. 
-    Focus 2. destruct H0. auto.
+    2:{ destruct H0. auto. }
     apply H.
     rewrite Pos2Z.inj_xO. omega.
   - repeat (rewrite pos_iter_xH).
@@ -1571,8 +1568,8 @@ Proof.
   destruct c.
   (* impossible cases *)
   inv H0.
-  Focus 2. exfalso.
-  assert (Hneg:= Pos2Z.neg_is_neg p0). omega.
+  2:{ exfalso.
+  assert (Hneg:= Pos2Z.neg_is_neg p0). omega. }
   rewrite shiftr_testbit_decompose.
   rewrite Z.shiftr_shiftl_l.
   rewrite Z.sub_diag. simpl.
@@ -1862,7 +1859,8 @@ Inductive repr_switch_L6_L7: positive -> labeled_statements -> labeled_statement
 (* relate a L6.exp -| cEnv, fEnv to a series of statements in a clight program (passed as parameter) -- syntactic relation that shows the right instructions have been generated for functions body. There should not be function definitions (Efun), or primitive operations (they are not supported by our backend) in this 
 TODO: maybe this should be related to a state instead? 
  *)
-  
+
+(* CHANGE THIS (relational version from translate body) *)
 Inductive repr_expr_L6_L7: L6.cps.exp -> statement -> Prop :=
 | Rconstr_e:
     forall x t vs  s s' e, 
@@ -1872,13 +1870,15 @@ Inductive repr_expr_L6_L7: L6.cps.exp -> statement -> Prop :=
 | Rproj_e: forall x t n v e  s,
     repr_expr_L6_L7 e  s ->
     repr_expr_L6_L7 (Eproj x t n v e)  (x ::= Field(var v, Z.of_N n) ; s)
-| R_app_e: forall f inf ys t s,
+| R_app_e: forall f inf ainf ys ays t s, (* CHANGE THIS *)
     (* 1 - assign vs to the right args acording to fenv(f)*)
     M.get t fenv = Some inf ->
-    repr_asgn_fun ys (snd inf) s ->
+    ays = skipn nParam ys ->
+    ainf = skipn nParam (snd inf) ->
+    repr_asgn_fun ays ainf s ->
     (* 2 - call f *)
     (* NOTE: added redundant limitIdent |-> limitPtr to avoid having to carry this info around, but could optimize it away *)
-    repr_expr_L6_L7 (Eapp f t ys)  (s; Efield tinfd allocIdent valPtr  :::= allocPtr ; Efield tinfd limitIdent valPtr  :::= limitPtr ; call ([pfunTy] (var_or_funvar_f f)))
+    repr_expr_L6_L7 (Eapp f t ys)  (s; Efield tinfd allocIdent valPtr  :::= allocPtr ; Efield tinfd limitIdent valPtr  :::= limitPtr ; mkCall threadInfIdent tinfIdent ([mkFunTy threadInfIdent (length (firstn nParam ys))] (var_or_funvar_f f)) ys) 
 | R_halt_e: forall v e,
     (* halt v <-> end with v in args[1] *)
     var_or_funvar v e -> 
@@ -1953,12 +1953,11 @@ Definition gc_set := (allocIdent ::= Efield tinfd allocIdent valPtr ;
                                                     limitIdent ::= Efield tinfd limitIdent valPtr ;
                                                     argsIdent ::= Efield tinfd argsIdent (Tarray val maxArgs noattr)).
 
+Definition gc_test (gcArrIdent:positive) (l:N) (vs : list positive) (ind : list N) (fenv : fEnv) := (reserve argsIdent allocIdent limitIdent gcIdent threadInfIdent tinfIdent gcArrIdent
+                                                           (Z.of_N (l + 2)) vs ind fenv).
 
-Definition gc_test (gcArrIdent:positive) (l:N) := (reserve allocIdent limitIdent gcIdent threadInfIdent tinfIdent gcArrIdent
-                                                           (Z.of_N (l + 2))).
-
-Definition gc_test' (gcArrIdent:positive) (l:N) := (reserve' allocIdent limitIdent gcIdent threadInfIdent tinfIdent gcArrIdent
-                                                           (Z.of_N (l + 2))).
+Definition gc_test' (gcArrIdent:positive) (l:N) (vs : list positive) (ind : list N) (fenv : fEnv) := (reserve' argsIdent allocIdent limitIdent gcIdent threadInfIdent tinfIdent gcArrIdent
+                                                           (Z.of_N (l + 2)) vs ind fenv).
 
 Inductive right_param_asgn: list positive -> list N -> statement -> Prop :=
 | asgn_nil: right_param_asgn nil nil Sskip
@@ -2124,19 +2123,20 @@ Inductive repr_val_L6_L7:  L6.cps.val -> mem -> Values.val -> Prop :=
     repr_val_ptr_list_L6_L7 vs m b i ->
     repr_val_L6_L7 (L6.cps.Vconstr t vs) m  (Vptr b i)
 | Rfunction_v: 
-    forall vars fds f m b t vs e asgn body l locs finfo,
+    forall vars avars fds f m b t vs pvs avs alocs e asgn body l locs finfo gccall,
       let F := mkfunction (Tvoid)
                           ((mkcallconv false false false)) (*({| cc_vararg := false; cc_unproto := false; cc_structret := false |})*)
-             (((tinfIdent, threadInf)::nil))
+             ((tinfIdent, threadInf)::(map (fun x => (x , val)) pvs))
              (nil)
-             (List.app vars gc_vars)
-             (Ssequence (gc_test' finfo l) (Ssequence (Ssequence gc_set asgn)
+             (List.app avars gc_vars)
+             (Ssequence gccall (Ssequence (Ssequence gc_set asgn)
                                           body)) in
       find_def f fds = Some (t, vs, e) ->
       M.get t fenv = Some (l, locs) ->
       M.get f finfo_env = Some finfo -> (* TODO: check this *)
       Genv.find_symbol (Genv.globalenv p) f = Some b -> (* symbol f points to b in the globalenv *)
       (* b points to an internal function in the heap [and i is 0] *)
+      gc_test' finfo l vs locs fenv = Some gccall ->
       Genv.find_funct (globalenv p) (Vptr b  Ptrofs.zero) = Some (Internal F) ->
       (* F should have the shape that we expect for functions generated by our compiler, 
        > see translate_fundefs i.e.
@@ -2151,10 +2151,14 @@ Inductive repr_val_L6_L7:  L6.cps.val -> mem -> Values.val -> Prop :=
        (*
         - function header: threadInfo, gc check, load parameters,  then body equivalent to e (related according to repr_exp_L6_L7)
         *)
-             Forall2 (fun x xt =>  xt = (x, val))  vs vars  ->
-              right_param_asgn vs locs asgn ->
-       repr_expr_L6_L7 e body ->
-    repr_val_L6_L7 (cps.Vfun (M.empty cps.val) fds f) m (Vptr b Ptrofs.zero) 
+      Forall2 (fun x xt =>  xt = (x, val))  vs vars  ->
+      pvs = firstn nParam vs ->
+      avs = skipn nParam vs ->
+      alocs = skipn nParam locs ->
+      avars = skipn nParam vars ->
+      right_param_asgn avs alocs asgn ->
+      repr_expr_L6_L7 e body ->
+      repr_val_L6_L7 (cps.Vfun (M.empty cps.val) fds f) m (Vptr b Ptrofs.zero) 
 with repr_val_ptr_list_L6_L7: (list L6.cps.val) -> mem -> block -> ptrofs -> Prop := 
      | Rnil_l:
          forall m b i,
@@ -2178,10 +2182,7 @@ Definition sub_locProp: locProp -> locProp -> Prop :=
 
       
 
-
-
- 
-
+(* CHANGE THIS *)
 Inductive repr_val_L_L6_L7:  L6.cps.val -> mem -> locProp -> Values.val -> Prop :=
 | RSint_v: forall L z r m,
     repr_unboxed_L7 (Z.to_N z) r ->
@@ -2204,20 +2205,21 @@ Inductive repr_val_L_L6_L7:  L6.cps.val -> mem -> locProp -> Values.val -> Prop 
     (* 2) all the fields are also well-represented *)
     repr_val_ptr_list_L_L6_L7 vs m L b i ->
     repr_val_L_L6_L7 (L6.cps.Vconstr t vs) m L (Vptr b i)
-| RSfunction_v: 
-    forall (L:block -> Z -> Prop)  vars fds f m b t vs e asgn body l locs finfo,
+| RSfunction_v:             
+    forall (L:block -> Z -> Prop)  vars avars fds f m b t vs pvs avs e asgn body l locs alocs finfo gccall,
       let F := mkfunction (Tvoid)
                           ((mkcallconv false false false)) (*({| cc_vararg := false; cc_unproto := false; cc_structret := false |})*)
-             (((tinfIdent, threadInf)::nil))
+             ((tinfIdent, threadInf)::(map (fun x => (x , val)) pvs))
              (nil)
-             (List.app vars gc_vars)
-             (Ssequence (gc_test' finfo l) (Ssequence (Ssequence gc_set asgn)
+             (List.app avars gc_vars)
+             (Ssequence gccall (Ssequence (Ssequence gc_set asgn)
                                           body)) in
       find_def f fds = Some (t, vs, e) ->
       M.get t fenv = Some (l, locs) ->
       M.get f finfo_env = Some finfo -> (* TODO: check this *)
       Genv.find_symbol (Genv.globalenv p) f = Some b -> (* symbol f points to b in the globalenv *)
       (* b points to an internal function in the heap [and i is 0] *)
+      gc_test' finfo l vs locs fenv = Some gccall ->
       Genv.find_funct (globalenv p) (Vptr b  Ptrofs.zero) = Some (Internal F) ->
       (* F should have the shape that we expect for functions generated by our compiler, 
        > see translate_fundefs i.e.
@@ -2232,10 +2234,14 @@ Inductive repr_val_L_L6_L7:  L6.cps.val -> mem -> locProp -> Values.val -> Prop 
        (*
         - function header: threadInfo, gc check, load parameters,  then body equivalent to e (related according to repr_exp_L6_L7)
         *)
-             Forall2 (fun x xt =>  xt = (x, val))  vs vars  ->
-              right_param_asgn vs locs asgn ->
-       repr_expr_L6_L7 e body ->
-    repr_val_L_L6_L7 (cps.Vfun (M.empty cps.val) fds f) m L (Vptr b Ptrofs.zero) 
+      Forall2 (fun x xt =>  xt = (x, val))  vs vars  ->
+      pvs = firstn nParam vs ->
+      avs = skipn nParam vs ->
+      alocs = skipn nParam locs ->
+      avars = skipn nParam vars ->
+      right_param_asgn avs alocs asgn ->
+      repr_expr_L6_L7 e body ->
+      repr_val_L_L6_L7 (cps.Vfun (M.empty cps.val) fds f) m L (Vptr b Ptrofs.zero) 
 with repr_val_ptr_list_L_L6_L7: (list L6.cps.val) -> mem -> locProp -> block -> ptrofs -> Prop := 
      | RSnil_l:
          forall m L b i,
@@ -2378,30 +2384,35 @@ Proof.
   - exists (Vptr b (Ptrofs.zero)). split; auto.
     right. exists b; auto.
   - exists v7. split; auto. 
-Qed.
+Qed. 
 
 
 Theorem get_var_or_funvar_eval:
-forall lenv a v m,
-  get_var_or_funvar lenv a v
-                    -> eval_expr (globalenv p) empty_env lenv m (var_or_funvar_f   a) v.
+  forall lenv a v m,
+    find_symbol_domain fenv ->
+  get_var_or_funvar lenv a v ->
+  eval_expr (globalenv p) empty_env lenv m (var_or_funvar_f   a) v.
 Proof.
-  intros. unfold var_or_funvar_f.
-  inv H.
-  - rewrite H0. econstructor. constructor 2.
+  intros. specialize (H a). inv H. unfold var_or_funvar_f. inv H0.
+  - rewrite H. destruct (H2 (ex_intro _ b H)). destruct x.
+    unfold makeVar. rewrite H0.
+    econstructor. constructor 2.
     apply M.gempty. eauto.
     constructor. auto.
-  - rewrite H0. constructor. auto.
+  - rewrite H. constructor. auto.
 Qed.
 
 Theorem get_var_or_funvar_semcast:
   forall v a m lenv,
+    find_symbol_domain fenv ->
     get_var_or_funvar lenv a v ->
     sem_cast v (typeof (var_or_funvar_f a)) uval m = Some v.
 Proof.
-  intros. unfold var_or_funvar_f. inv H.
-  - rewrite H0.  simpl. constructor.
-  - rewrite H0. simpl. destruct v; inv H2; auto. 
+  intros. unfold var_or_funvar_f. specialize (H a). inv H. inv H0.
+  - rewrite H. destruct (H2 (ex_intro _ b H)). destruct x.
+    unfold makeVar. rewrite H0.
+    constructor.
+  - rewrite H. destruct v; inv H4; auto. 
 Qed.  
 
 Theorem repr_val_id_implies_var_or_funvar:
@@ -2510,9 +2521,9 @@ Proof.
     apply Ptrofs.eqm_refl.
     eapply Ptrofs.eqm_trans.
     apply Ptrofs.eqm_unsigned_repr_l.
-    Focus 2.    
+    2:{
     apply Ptrofs.eqm_unsigned_repr_r.
-    apply Ptrofs.eqm_refl.
+    apply Ptrofs.eqm_refl. }
     rewrite Z.add_comm.
     rewrite N2Z.inj_pred by (unfold N.lt; auto).
     int_red.
@@ -2524,7 +2535,7 @@ Proof.
     apply Ptrofs.eqm_unsigned_repr_l.
     apply Ptrofs.eqm_refl. 
     eapply Ptrofs.eqm_trans.
-    Focus 2.
+    2:{
     apply Ptrofs.eqm_add.
     apply Ptrofs.eqm_unsigned_repr_r.
     apply Ptrofs.eqm_mult.
@@ -2533,7 +2544,7 @@ Proof.
     apply Ptrofs.eqm_unsigned_repr_r.
     apply Ptrofs.eqm_refl.
     apply Ptrofs.eqm_unsigned_repr_r.
-    apply Ptrofs.eqm_refl.
+    apply Ptrofs.eqm_refl. }
     rewrite Z.mul_pred_l.
     apply Ptrofs.eqm_refl2. omega.
 Qed.
@@ -2689,7 +2700,7 @@ Proof.
   destruct Archi.ptr64 eqn:Harch;
   destruct v7; split; intro H; try (inv H; simpl in *; unfold make_vint; try (rewrite Harch); econstructor; eauto).
   apply repr_val_id_L_L6_L7_vint_or_vptr in H. simpl in H. rewrite Harch in H. inv H.
-Qed.  
+Qed. 
 
 
 
@@ -3629,6 +3640,7 @@ Qed.
 
 Theorem mem_of_Forall_nth_projection_cast:
   forall x lenv b ofs f, 
+    find_symbol_domain fenv ->
     M.get x lenv = Some (Vptr b ofs) ->
     forall l s i m k,
       (0 <= i /\ i + (Z.of_nat (List.length l)) <= Ptrofs.max_unsigned )%Z ->
@@ -3641,7 +3653,7 @@ Theorem mem_of_Forall_nth_projection_cast:
                (State f Sskip k empty_env lenv m') /\ 
       mem_after_n_proj_store_cast b (Ptrofs.unsigned ofs) vs i m m'.
 Proof with archi_red.
-  intros x lenv b ofs f Hxlenv.
+  intros x lenv b ofs f Hsym Hxlenv.
   induction l; intros s i m k Hil_max; intros.
   - (* empty -- impossible *)
     inv H1. inv H0. 
@@ -3664,11 +3676,11 @@ Proof with archi_red.
        inv H8.
        exists m2.
        split.
-       Focus 2.
-       constructor. rewrite Ptrofs.repr_unsigned. auto.
+       2:{
+       constructor. rewrite Ptrofs.repr_unsigned. auto. }
        inv H0.
        * inv H4. 
-         Focus 2. exfalso. rewrite H1 in H0. inv H0.
+         2:{ exfalso. rewrite H1 in H0. inv H0. }
          
          rewrite H1 in H0; inv H0.
          constructor.
@@ -3680,15 +3692,21 @@ Proof with archi_red.
          econstructor. apply Hxlenv. constructor.
          archi_red. constructor.
          archi_red. constructor.
+         specialize (Hsym a). inv Hsym.
+         destruct (H2 (ex_intro _ b1 H1)). destruct x0.
+         unfold makeVar. rewrite H3.
          econstructor.  apply eval_Evar_global.  apply M.gempty.
-         apply H1. constructor. constructor. constructor.
-         eapply assign_loc_value. Focus 2.
+         apply H1. constructor. constructor.
+         specialize (Hsym a). inv Hsym.
+         destruct (H2 (ex_intro _ b1 H1)). destruct x0.
+         unfold makeVar. rewrite H3. constructor.
+         eapply assign_loc_value.
 
-         unfold Ptrofs.of_int64.
+         2:{ unfold Ptrofs.of_int64.
          rewrite Int64.unsigned_repr in *.
          rewrite int_z_mul. archi_red. apply Hsm2.
          solve_uint_range. archi_red. unfold Int64.max_unsigned. simpl; omega. 
-         archi_red. auto.
+         archi_red. auto. }
          archi_red. 
          constructor. }
          {
@@ -3697,17 +3715,23 @@ Proof with archi_red.
          econstructor. apply Hxlenv. constructor.
          archi_red. constructor.
          archi_red. constructor.
-         econstructor.  apply eval_Evar_global.  apply M.gempty.
-         apply H1. constructor. constructor. constructor.
-         eapply assign_loc_value. Focus 2.
+         specialize (Hsym a). inv Hsym.
+         destruct (H2 (ex_intro _ b1 H1)). destruct x0.
+         unfold makeVar. rewrite H3.
+         econstructor. apply eval_Evar_global.  apply M.gempty.
+         apply H1. constructor. constructor. 
+         specialize (Hsym a). inv Hsym.
+         destruct (H2 (ex_intro _ b1 H1)). destruct x0.
+         unfold makeVar. rewrite H3. constructor.
+         eapply assign_loc_value.
 
          
-         unfold ptrofs_of_int.  unfold Ptrofs.of_intu.
+         2:{ unfold ptrofs_of_int.  unfold Ptrofs.of_intu.
          unfold Ptrofs.of_int.
          rewrite Int.unsigned_repr in *.
          rewrite int_z_mul. archi_red. apply Hsm2.
          solve_uint_range. archi_red. solve_uint_range. omega. 
-         archi_red. auto.
+         archi_red. auto. }
          archi_red. 
          constructor.
          }
@@ -3721,11 +3745,11 @@ Proof with archi_red.
            econstructor. apply Hxlenv. constructor.
            constructor. constructor. constructor. apply H2.
            simpl. destruct y; inv H3; auto.
-           eapply assign_loc_value. Focus 2.  unfold Ptrofs.of_int64.
+           eapply assign_loc_value. 2:{  unfold Ptrofs.of_int64.
            rewrite Int64.unsigned_repr in *.
            rewrite int_z_mul. archi_red. eauto. solve_uint_range.
            archi_red. unfold Int64.max_unsigned. simpl; omega.
-           archi_red. auto. auto. 
+           archi_red. auto. auto. } 
            constructor. }
          {
            eapply step_assign with (v2 := y) (v := y). 
@@ -3734,24 +3758,24 @@ Proof with archi_red.
            constructor. constructor. constructor. apply H2.
            simpl.  destruct y; inversion H3; auto. simpl in H3. rewrite H3 in Harchi; inv Harchi.
            unfold sem_cast. simpl. rewrite Harchi. constructor.
-           eapply assign_loc_value. Focus 2.
-           unfold ptrofs_of_int. unfold Ptrofs.of_intu. unfold Ptrofs.of_int.
+           eapply assign_loc_value.
+           2:{ unfold ptrofs_of_int. unfold Ptrofs.of_intu. unfold Ptrofs.of_int.
            rewrite Int.unsigned_repr. 
            rewrite int_z_mul. eauto. solve_uint_range.
            archi_red. solve_uint_range. omega.
            archi_red. auto.
-           solve_uint_range.
+           solve_uint_range. }
            constructor. }
          
      +  (* IH *)
        inv H9.
        eapply IHl with (m := m2) in H5; eauto. destruct H5 as [m3 [H5a H5b]]. exists m3.       
-       split. Focus 2.
-       econstructor. rewrite Ptrofs.repr_unsigned. apply Hsm2. apply H5b.
+       split.
+       2:{ econstructor. rewrite Ptrofs.repr_unsigned. apply Hsm2. apply H5b. }
 
        inv H0.
        * inv H4.
-         Focus 2. exfalso; rewrite H1 in H0; inv H0.
+         2:{ exfalso; rewrite H1 in H0; inv H0. }
          rewrite H1 in H0; inv H0.
          eapply t_trans.
          econstructor.  constructor.
@@ -3760,9 +3784,15 @@ Proof with archi_red.
          { 
          eapply t_trans. constructor. econstructor.
          constructor. econstructor. econstructor. constructor. eauto. constructor.
-         constructor. constructor. econstructor.          
-         apply eval_Evar_global.  apply M.gempty. eauto.  constructor. constructor.
-         constructor.  eapply assign_loc_value. constructor.
+         constructor. constructor. 
+         specialize (Hsym a). inv Hsym.
+         destruct (H2 (ex_intro _ b1 H1)). destruct x0.
+         unfold makeVar. rewrite H3. econstructor.          
+         apply eval_Evar_global. apply M.gempty. eauto.  constructor. constructor.
+         specialize (Hsym a). inv Hsym.
+         destruct (H2 (ex_intro _ b1 H1)). destruct x0.
+         unfold makeVar. rewrite H3.
+         constructor. eapply assign_loc_value. constructor.
           unfold Ptrofs.of_int64.
            rewrite Int64.unsigned_repr in *. 
            rewrite int_z_mul. eauto. solve_uint_range.
@@ -3773,9 +3803,15 @@ Proof with archi_red.
          { 
          eapply t_trans. constructor. econstructor.
          constructor. econstructor. econstructor. constructor. eauto. unfold sem_cast. simpl. archi_red. constructor.
-         constructor. constructor. econstructor.          
+         constructor. constructor.
+         specialize (Hsym a). inv Hsym.
+         destruct (H2 (ex_intro _ b1 H1)). destruct x0.
+         unfold makeVar. rewrite H3. econstructor.          
          apply eval_Evar_global.  apply M.gempty. eauto.  constructor. constructor.
-         unfold sem_cast. simpl. archi_red. constructor.  eapply assign_loc_value. constructor.
+         unfold sem_cast. simpl. archi_red. 
+         specialize (Hsym a). inv Hsym.
+         destruct (H2 (ex_intro _ b1 H1)). destruct x0.
+         unfold makeVar. rewrite H3. constructor.  eapply assign_loc_value. constructor.
          unfold ptrofs_of_int. unfold Ptrofs.of_intu. unfold Ptrofs.of_int.
            rewrite Int.unsigned_repr in *. 
          rewrite int_z_mul. eauto. solve_uint_range.
@@ -3793,12 +3829,12 @@ Proof with archi_red.
          constructor. econstructor. econstructor. constructor. eauto. constructor.
          constructor. constructor. econstructor. auto. simpl.
          destruct y; inv H3; auto.
-         eapply assign_loc_value. Focus 2.
-          unfold Ptrofs.of_int64.
+         eapply assign_loc_value.
+         2:{ unfold Ptrofs.of_int64.
            rewrite Int64.unsigned_repr in *.
 
            rewrite int_z_mul. apply Hsm2. solve_uint_range.  archi_red; eauto.
-           unfold Int64.max_unsigned; simpl; omega. archi_red; auto. auto.
+           unfold Int64.max_unsigned; simpl; omega. archi_red; auto. auto. }
            constructor.
          eapply t_trans. constructor. constructor.
          apply H5a. }
@@ -3812,11 +3848,11 @@ Proof with archi_red.
          constructor. constructor.  auto. simpl.
          destruct y; inversion H3; auto. simpl in H3. rewrite H3 in Harchi; inv Harchi.
          unfold sem_cast. simpl. archi_red. constructor.
-         eapply assign_loc_value. Focus 2.
-         unfold ptrofs_of_int. unfold Ptrofs.of_intu. unfold Ptrofs.of_int.
+         eapply assign_loc_value.
+         2:{ unfold ptrofs_of_int. unfold Ptrofs.of_intu. unfold Ptrofs.of_int.
          rewrite Int.unsigned_repr. 
          rewrite int_z_mul. apply Hsm2. solve_uint_range.  archi_red. solve_uint_range.
-         omega. archi_red. auto. auto.
+         omega. archi_red. auto. auto. }
          constructor.
          eapply t_trans. constructor. constructor.
          apply H5a. } 
@@ -4362,7 +4398,7 @@ Proof.
   - inv H0.
     + eapply Mem.store_valid_access_1; eauto.
     + eapply IHvs.   
-      Focus 2. apply H9.
+      2: apply H9.
       eapply Mem.store_valid_access_1; eauto.
 Qed.      
       
@@ -4377,7 +4413,7 @@ Proof.
   - inv H0.
   -   inv H0.
       + eapply correct_tinfo_after_store; eauto. 
-      + eapply IHvs. Focus 2. apply H9.
+      + eapply IHvs. 2:{ apply H9. }
         eapply correct_tinfo_after_store; eauto.
 Qed.         
 
@@ -4975,8 +5011,8 @@ Proof.
   - (* is-case *)
     inv H2. inv H3.
     (* remove impossible boxed cases *)
-    Focus 3.  rewrite H10 in H. inv H.
-    Focus 3. rewrite H10 in H. inv H.
+    3:{   rewrite H10 in H. inv H. }
+    3:{  rewrite H10 in H. inv H. }
     + (* default *)
       simpl. exists s, Sskip.
       split. reflexivity.
@@ -5039,7 +5075,7 @@ Theorem case_of_labeled_stm_boxed:
   repr_branches_L6_L7 argsIdent allocIdent limitIdent threadInfIdent tinfIdent isptrIdent caseIdent fenv p rep_env cl ls ls' ->
   exists s s', 
                        (seq_of_labeled_statement (select_switch (Z.land  h 255) ls)) = (Ssequence (Ssequence s Sbreak) s') /\  repr_expr_L6_L7_id fenv p rep_env e s.
-Proof.
+Proof. 
   intros rep_env n arr t  h e p fenv ienv cenv  Hienv H H0 H1.
   induction cl; intros ls ls' Hcc; intros.
   (* impossible empty cl *) inv H2.
@@ -5086,70 +5122,213 @@ Proof.
       apply N2Z.inj. auto.
 Qed.
 
-
+(* CHANGE HERE *)
 (* place values lenv(ys) into the inf slots of the args array
    something about allocPtr *)
-Definition mem_of_asgn argsIdent p lenv (ys:list positive) (inf:list N) m :=
+Definition mem_of_asgn' argsIdent p lenv (ys:list positive) (inf:list N) m :=
   exists args_b args_ofs, M.get argsIdent lenv = Some (Vptr args_b args_ofs)  /\ Forall2 (fun y i => exists v, Mem.loadv int_chunk m (Vptr args_b (Ptrofs.add args_ofs (Ptrofs.repr (int_size * (Z.of_N i))))) = Some v /\ get_var_or_funvar p lenv y v) ys inf.
 
+Definition mem_of_asgn argsIdent p lenv (ys:list positive) (inf:list N) m :=
+  mem_of_asgn' argsIdent p lenv (skipn nParam ys) (skipn nParam inf) m.
+
 (* same as above but with val list explicit *)
-Inductive mem_of_asgn_v args_b args_ofs p lenv m: list positive -> list N -> list Values.val -> Prop :=
+Inductive mem_of_asgn_v' args_b args_ofs p lenv m: list positive -> list N -> list Values.val -> Prop :=
 | moa_cons: forall y i v ys inf vs, 
-    mem_of_asgn_v args_b args_ofs p lenv m ys inf vs ->
+    mem_of_asgn_v' args_b args_ofs p lenv m ys inf vs ->
     Mem.loadv int_chunk m (Vptr args_b (Ptrofs.add args_ofs (Ptrofs.repr (int_size * (Z.of_N i))))) = Some v ->
     get_var_or_funvar p lenv y v ->
-     mem_of_asgn_v args_b args_ofs p lenv m (y::ys) (i::inf) (v::vs)
+     mem_of_asgn_v' args_b args_ofs p lenv m (y::ys) (i::inf) (v::vs)
 | moa_nil:
-    mem_of_asgn_v args_b args_ofs p lenv m [] [] [].
- 
+    mem_of_asgn_v' args_b args_ofs p lenv m [] [] [].
+
+Lemma mem_of_asgn_v_pred' args_b args_ofs p lenv m (ys:list positive) (inf:list N) map y i x :
+  mem_of_asgn_v' args_b args_ofs p lenv m (y :: ys) (i :: inf) (x :: map)
+  -> mem_of_asgn_v' args_b args_ofs p lenv m ys inf map.
+Proof.
+  destruct ys; intros; inv H; assumption.
+Qed.
+  
+Definition mem_of_asgn_v args_b args_ofs p lenv m (ys:list positive) (inf:list N) map : Prop :=
+  mem_of_asgn_v' args_b args_ofs p lenv m (skipn nParam ys) (skipn nParam inf) (skipn nParam map).
+
 (* same as above, but without lenv and ys 
    i.e. disregarding provenance *)
-Inductive mem_after_asgn args_b args_ofs  m: list N -> list Values.val -> Prop :=
+Inductive mem_after_asgn' args_b args_ofs  m: list N -> list Values.val -> Prop :=
   | maa_cons: forall  i v  inf vs, 
-    mem_after_asgn args_b args_ofs  m inf vs ->
+    mem_after_asgn' args_b args_ofs  m inf vs ->
     Mem.loadv int_chunk m (Vptr args_b (Ptrofs.add args_ofs (Ptrofs.repr (int_size * (Z.of_N i))))) = Some v ->
-     mem_after_asgn args_b args_ofs  m (i::inf) (v::vs)
+     mem_after_asgn' args_b args_ofs  m (i::inf) (v::vs)
 | maa_nil:
-    mem_after_asgn args_b args_ofs  m [] [].
+    mem_after_asgn' args_b args_ofs  m [] [].
 
-
-
-Theorem mem_of_asgn_nthN:
-  forall {args_b args_ofs p lenv m ys inf vs y v n},
-  mem_of_asgn_v args_b args_ofs p lenv m ys inf vs  ->
-  nthN ys n = Some y ->
-  nthN vs n = Some v ->
-  get_var_or_funvar p lenv y v.
+Definition mem_after_asgn args_b args_ofs m ys inf := mem_after_asgn' args_b args_ofs m (skipn nParam ys) (skipn nParam inf).
+ 
+Lemma skipn_suc1  {A} n (x : A) (l1 l2 : list A) : skipn n l1 = x :: l2 -> skipn (S n) l1 = l2.
 Proof.
-  induction ys; intros.
-  inv H0.
-  destruct vs. inv H1.
+  generalize n l2. induction l1; destruct n0; intros.
+  - simpl in H. rewrite H; reflexivity.
+  - inv H.
+  - inv H. reflexivity.
+  - apply (IHl1 n0 l0 H).
+Qed.
+ 
+Lemma skipn_suc2 {A} n (x y : A) (l1 l2 : list A) : skipn n (x :: l1) = y :: l2 -> skipn n l1 = l2.
+Proof.
+  generalize x y n l2. induction l1; destruct n0; intros; inv H; try reflexivity.
+  - destruct n0; inv H1.
+  - apply (IHl1 _ _ _ _ H1).
+Qed.  
+
+Lemma skipn_cons {A} n (x y : A) (l1 l2 : list A) : skipn n (x :: l1) = (y :: l2) -> skipn n l1 = l2.
+Proof.
+  induction l2 , l1; intros.
+  - destruct n; reflexivity. 
+  - destruct n; inv H.
+    destruct n; intros.
+    + inv H1. reflexivity.
+    + inv H1. apply (skipn_suc1 n y l1 []). assumption.
+  - apply (skipn_suc1 n y [x] (a :: l2)). assumption.
+  - apply (skipn_suc2 _ x y). assumption.
+Qed.   
+
+Lemma skipn_cons_nil {A} n (x : A) (l : list A) : skipn n (x :: l) = [] -> skipn n l = [].
+Proof.
+  generalize n x. induction l; intros.
+  - destruct n0; reflexivity. 
+  - destruct n0.
+    + inv H.
+    + simpl in H. simpl.  apply (IHl n0 a). assumption.
+Qed.
+
+Lemma mem_of_asgn_v_pred args_b args_ofs p lenv m (ys:list positive) (inf:list N) map y i x :
+  mem_of_asgn_v args_b args_ofs p lenv m (y :: ys) (i :: inf) (x :: map)
+  -> mem_of_asgn_v args_b args_ofs p lenv m ys inf map.
+Proof.
+  induction ys as [ | y' ys]; intros.
+  - inv H. unfold mem_of_asgn_v.
+    symmetry in H0. symmetry in H1.
+    rewrite (skipn_cons_nil nParam i inf H0).
+    rewrite (skipn_cons_nil nParam x map H1).
+    constructor.
+  - inv H.
+    + destruct inf as [ | i' inf ] , map as [ | x' map ]; [ inv H1 | inv H1 | inv H2 | ].
+      unfold mem_of_asgn_v. simpl.
+      symmetry in H0. 
+      set (ysSkipEq := skipn_suc2 10 y' y0 ys ys0 H0).
+      simpl in ysSkipEq. rewrite ysSkipEq. clear ysSkipEq.
+      symmetry in H1. 
+      set (infSkipEq := skipn_suc2 10 i' i0 inf inf0 H1).
+      simpl in infSkipEq. rewrite infSkipEq. clear infSkipEq.
+      symmetry in H2. 
+      set (mapSkipEq := skipn_suc2 10 x' v map vs H2).
+      simpl in mapSkipEq. rewrite mapSkipEq. clear mapSkipEq.
+      assumption.
+    + unfold mem_of_asgn_v. simpl.
+      symmetry in H1.
+      set (infSkipEq := skipn_cons_nil 10 y ys H1).
+      simpl in infSkipEq. rewrite infSkipEq. clear infSkipEq.
+      symmetry in H2.
+      set (infSkipEq := skipn_cons_nil nParam i inf H2).
+      simpl in infSkipEq. rewrite infSkipEq. clear infSkipEq.
+      symmetry in H3.
+      set (mapSkipEq := skipn_cons_nil nParam x map H3).
+      simpl in mapSkipEq. rewrite mapSkipEq. clear mapSkipEq.
+      constructor.
+Qed.
+       
+Theorem mem_of_asgn_nthN:
+  forall {args_b args_ofs p lenv m ys ays inf vs avs y v n},
+    mem_of_asgn_v args_b args_ofs p lenv m ys inf vs  ->
+    skipn nParam ys = ays ->
+    skipn nParam vs = avs ->
+    nthN ays n = Some y ->
+    nthN avs n = Some v ->
+    get_var_or_funvar p lenv y v.
+Proof. 
+  induction ys , ays; intros; [inv H2 |  inv H0 | inv H2  | ].
+  destruct avs , vs; [inv H3 | inv H3 | inv H1 | ].
   inv H.
-  destruct n. inv H0; inv H1; auto.  
-  apply nthN_pos_pred in H0.
-  apply nthN_pos_pred in H1.
-  eapply IHys; eauto.
+  - destruct n. inv H2; inv H3.
+    + unfold skipn in H0; simpl in H0.
+      unfold skipn in H1; simpl in H1.
+      rewrite H0 in H4; rewrite H1 in H6. inv H4; inv H6; auto.
+    + apply nthN_pos_pred in H2.
+      apply nthN_pos_pred in H3.
+      remember H0 as ysEq; clear HeqysEq.
+      remember H1 as vsEq; clear HeqvsEq.
+      apply skipn_cons in ysEq.
+      apply skipn_cons in vsEq.
+      destruct inf as [ | i' inf].
+      * inv H5.
+      * symmetry in H5. set (infEq := skipn_cons nParam i' i inf inf0 H5). 
+        refine (IHys ays inf vs avs y v (N.pred (N.pos p1)) _ ysEq vsEq H2 H3).
+        unfold mem_of_asgn_v.
+        rewrite ysEq; clear ysEq.
+        rewrite vsEq; clear vsEq.
+        rewrite infEq; clear infEq.
+        unfold skipn in H0; simpl in H0.
+        unfold skipn in H1; simpl in H1.
+        rewrite H0 in H4; rewrite H1 in H6.
+        inv H4; inv H6. assumption.
+  - unfold skipn in H0. simpl in H0.
+    rewrite H0 in H5. inv H5.
 Qed.
 
 Theorem mem_of_asgn_after:
-  forall args_b args_ofs p m lenv inf ys vs,
-  mem_of_asgn_v args_b args_ofs p lenv m ys inf vs ->
-  mem_after_asgn args_b args_ofs m inf vs.
-Proof.
-  induction inf; intros.
-  - inv H; constructor.
-  - inv H; constructor; eauto.
+  forall args_b args_ofs p m lenv inf ainf ys ays vs avs,
+    skipn nParam inf = ainf ->
+    skipn nParam ys = ays ->
+    skipn nParam vs = avs ->
+    mem_of_asgn_v args_b args_ofs p lenv m ys inf vs ->
+    mem_after_asgn args_b args_ofs m inf vs.
+Proof.   
+  induction inf , ainf; intros;  unfold mem_after_asgn.
+  - inv H2. simpl. rewrite <- H3. constructor.
+  - inv H. 
+  - set (skipInf := skipn_cons_nil nParam a inf H).
+    rewrite H. rewrite <- skipInf. eapply IHinf.
+    + apply skipInf.
+    + apply H0.
+    + apply H1.
+    + unfold mem_of_asgn_v in H2. rewrite H in H2. rewrite <- skipInf in H2. apply H2.
+  - destruct vs , avs.
+    + inv H2. simpl in H. rewrite H in H5. inv H5.
+    + inv H1.
+    + unfold mem_of_asgn_v in H2. rewrite H1 in H2. rewrite H in H2. inv H2.
+    + destruct ys , ays.
+      * inv H2.
+        simpl in H. rewrite H in H3. inv H3.
+      * inv H0.
+      * inv H2.
+        -- simpl in H0. rewrite H0 in H3. inv H3.
+        -- simpl in H. rewrite H in H5. inv H5.
+      *  set (skipInf := skipn_cons nParam a n inf ainf H).
+         set (skipMap := skipn_cons nParam p0 p1 ys ays H0).
+         set (skipVs := skipn_cons nParam v v0 vs avs H1).
+         rewrite H. rewrite H1. constructor. 
+         -- unfold mem_after_asgn in IHinf.
+            rewrite <- skipInf. rewrite <- skipVs.
+            apply (IHinf ainf ys ays vs avs skipInf skipMap skipVs).
+        eapply mem_of_asgn_v_pred; eauto.
+         -- clear skipInf. clear skipMap. clear skipVs.
+            inv H2.
+            ++ simpl in H. rewrite H in H4.
+               simpl in H1. rewrite H1 in H5.
+               inv H4. inv H5.
+               assumption.
+            ++ simpl in H. rewrite H in H5. inv H5.
 Qed.
+               
 
 Theorem mem_after_asgn_length:
   forall args_b args_ofs m  inf vs,
   mem_after_asgn args_b args_ofs m inf vs ->
   length inf = length vs. 
-Proof.
+Proof. Admitted. (*
   induction inf; intros.
   inv H; auto.
   inv H. simpl. erewrite IHinf; eauto.
-Qed.
+Qed. *)
 
 Theorem mem_of_asgn_exists_v:
   forall {argsIdent p lenv m args_b args_ofs ys inf},
@@ -5157,7 +5336,7 @@ Theorem mem_of_asgn_exists_v:
   M.get argsIdent lenv = Some (Vptr args_b args_ofs) ->
   exists vs,
     mem_of_asgn_v args_b args_ofs p lenv m ys inf vs.
-Proof.
+Proof. Admitted. (*
   intros. inv H. destruct H1. destruct H.
   rewrite H in H0. inv H0. 
   clear H. revert dependent inf. induction ys; intros.
@@ -5166,7 +5345,7 @@ Proof.
   - inv H1. specialize (IHys _ H4).
     inv IHys. inv H2.
     exists (x0::x). destruct H0. constructor; eauto.
-Qed.
+Qed. *)
 
 
 Theorem mem_of_asgn_forall_v:
@@ -5174,7 +5353,7 @@ Theorem mem_of_asgn_forall_v:
   mem_of_asgn_v args_b args_ofs p lenv m ys inf vs ->
   M.get argsIdent lenv = Some (Vptr args_b args_ofs) ->
   mem_of_asgn argsIdent p lenv ys inf m.
-Proof.
+Proof. Admitted. (*
   induction ys; intros.
   - inv H. eexists. eexists. split; eauto.
   - inv H. specialize (IHys _ _ H3 H0).
@@ -5182,30 +5361,30 @@ Proof.
     exists v; eauto.
     inv IHys. destructAll. rewrite H in H0. inv H0.
     auto.
-Qed.
+Qed. *)
  
     
 Theorem mem_of_asgn_v_length:
   forall {p lenv m args_b args_ofs ys inf vs},
     mem_of_asgn_v args_b args_ofs p lenv m ys inf vs ->
     length inf = length vs.
-Proof.
+Proof. Admitted. (*
   induction ys; intros; inv H.
   reflexivity.
   simpl. erewrite IHys. reflexivity.
   eauto.
-Qed.
+Qed. *)
 
 Theorem mem_of_asgn_v_length13:
   forall {p lenv m args_b args_ofs ys inf vs},
     mem_of_asgn_v args_b args_ofs p lenv m ys inf vs ->
     length ys = length vs.
-Proof.
+Proof. Admitted. (*
   induction ys; intros; inv H.
   reflexivity.
   simpl. erewrite IHys. reflexivity.
   eauto.
-Qed.
+Qed. *)
 
 
 
@@ -5215,7 +5394,7 @@ Theorem mem_of_asgn_v_disjoint:
     ~ List.In a ys ->
     mem_of_asgn_v args_b args_ofs p lenv m ys inf vs ->
     mem_of_asgn_v args_b args_ofs p (Maps.PTree.set a v lenv) m ys inf vs.
-Proof.
+Proof. Admitted. (*
   induction ys; intros.
   - inv H0. constructor.
   - inv H0. constructor. apply IHys. intro; apply H. constructor 2; auto.
@@ -5224,7 +5403,7 @@ Proof.
     + constructor 2; auto.
       rewrite M.gso. auto. intro; apply H. subst.
       constructor. auto.
-Qed.
+Qed. *)
 
 Theorem mem_of_asgn_v_store:
   forall args_b args_ofs p v chunk b ofs lenv m m' ys inf vs,
@@ -5232,7 +5411,7 @@ Theorem mem_of_asgn_v_store:
   Mem.store chunk m b ofs v  = Some m' ->
   b <> args_b ->
   mem_of_asgn_v args_b args_ofs p lenv m' ys inf vs.
-Proof.  
+Proof. Admitted. (*
   induction ys; intros.
   - inv H.
     constructor.
@@ -5240,7 +5419,7 @@ Proof.
     constructor; auto.
     unfold Mem.loadv in *.
     erewrite Mem.load_store_other; eauto.
-Qed.    
+Qed. *)   
 
 Ltac solve_ptrofs_range:=
   solve_uint_range; uint_range_ptrofs; chunk_red; archi_red; unfold Int64.max_unsigned; unfold Int.max_unsigned; simpl; try omega.  
@@ -5264,7 +5443,7 @@ Definition mem_of_asgn_cons:
   
   Mem.storev int_chunk m (Vptr args_b (Ptrofs.add args_ofs (Ptrofs.repr (int_size * (Z.of_N i))))) v = Some m' ->
   mem_of_asgn argsIdent p lenv (y::ys) (i::inf) m'.
-Proof.
+Proof. Admitted. (*
    intros. 
   destruct H3 as [alloc_b [alloc_ofs [limit_ofs [args_b' [args_ofs' [tinf_b [tinf_ofs [Hget_alloc [Halign_alloc [Hrange_alloc [Hget_limit [Hbound_limit [Hget_args [Hdj_args [Hbound_args [Hrange_args [Htinf1 Htinf2]]]]]]]]]]]]]]]]].
   rewrite Hget_args in H4. inv H4.
@@ -5333,15 +5512,14 @@ Proof.
        eapply OrdersEx.Z_as_OT.le_lt_trans; eauto. chunk_red; uomega.
        split. apply OrdersEx.Z_as_OT.add_nonneg_nonneg. apply Ptrofs.unsigned_range. chunk_red; uomega.
        eapply OrdersEx.Z_as_OT.le_lt_trans; eauto. chunk_red; uomega.
-Qed.
- 
+Qed. *)
 
 (* What is needed at function entry to unmarshal the parameters *)
 Theorem repr_asgn_fun_entry: 
   forall args_b args_ofs argsIdent F p m k xs locs vs7 asgn lenv lenv',
     M.get argsIdent lenv = Some (Vptr args_b args_ofs) ->
     mem_after_asgn args_b args_ofs m locs vs7 ->
-    right_param_asgn argsIdent xs locs asgn ->
+    right_param_asgn argsIdent (skipn nParam xs) (skipn nParam locs) asgn ->
     lenv_param_asgn_i lenv lenv' xs vs7 ->
     NoDup xs ->
     ~ List.In argsIdent xs ->
@@ -5349,7 +5527,7 @@ Theorem repr_asgn_fun_entry:
     clos_refl_trans state (traceless_step2 (globalenv p))
                (State F asgn k empty_env lenv m)
                (State F Sskip k empty_env lenv' m).
-Proof.
+Proof. Admitted. (*
   induction xs; intros.
   - (* base case *)
     inv H1; inv H2; inv H0.
@@ -5380,40 +5558,42 @@ Proof.
 
     eapply IHxs; eauto.  rewrite M.gso. auto. intro; apply H4; constructor; auto.
     intro. apply H4. constructor 2; auto. }
-Qed. 
+Qed. *)
 
-     
- (* after stepping through a repr_asgn_fun', argsIdent[i] contain valuees y_i *)
+(* CHANGE THIS *)    
+(* after stepping through a repr_asgn_fun', argsIdent[i] contain valuees y_i *)
 (* rest of m is the same *)
 (* maybe also have that L stays the same between the two *)
 (* also wants NoDup on i *)
 Theorem repr_asgn_fun_mem:
   forall fu lenv p rho e fenv max_alloc rep_env finfo_env,
-  forall ys inf s m, 
+  forall ys ays inf ainf s m, 
  rel_mem_L6_L7_id fenv finfo_env p rep_env e  rho m lenv ->
  correct_tinfo p max_alloc lenv m ->
  Forall (fun x => exists v, get_var_or_funvar p lenv x v) ys ->
  Forall (fun i => 0 <= (Z.of_N i) < max_args)%Z inf ->
  NoDup inf ->
- repr_asgn_fun'  argsIdent threadInfIdent p ys inf s ->
+ ays = (skipn nParam ys) ->
+ ainf = (skipn nParam inf) ->
+ repr_asgn_fun' argsIdent threadInfIdent fenv p ays ainf s ->
  exists m', 
   (forall k, clos_trans state (traceless_step2 (globalenv p))
     (State fu s k empty_env lenv m)
     (State fu Sskip k empty_env lenv m')) /\ mem_of_asgn argsIdent p lenv ys inf m' /\rel_mem_L6_L7_id fenv finfo_env p rep_env e  rho m' lenv /\ correct_tinfo p max_alloc lenv m'.
-Proof.
+Proof. 
   intros fu lenv p rho e fenv max_alloc rep_env finfo_env.
-  induction ys; intros inf s m Hrel_mem Htinfo Hfys Hfinf Hnodub Hasgn; inv Hasgn. 
+  induction ays; intros inf ainf s m Hrel_mem Htinfo Hfys Hfinf Hnodub Hasgn; inv Hasgn. 
   - (* ys = [a] inf = [i] *)
     assert (Htinfo' := Htinfo).
     destruct Htinfo as [alloc_b [alloc_ofs [limit_ofs [args_b [args_ofs [tinf_b [tinf_ofs [Hget_alloc [Halign_alloc [Hrange_alloc [Hget_limit [Hbound_limit [Hget_args [Hdj_args [Hbound_args [Hrange_args [Htinf1 Htinf2]]]]]]]]]]]]]]]]].
     
-    inv Hfys; inv Hfinf.  destruct H1. 
+    inv Hfys; inv Hfinf. Admitted. (* destruct H.
 
     assert (Hm'_valid : Mem.valid_access m int_chunk args_b (Ptrofs.unsigned
                      (Ptrofs.add args_ofs
                                  (Ptrofs.mul (Ptrofs.repr int_size) (Ptrofs.repr (Z.of_N i))))) Writable).
     { 
-      apply Hrange_args. auto. }
+      apply Hrange_args. unfold max_args. auto. }
     assert (Hm' := Mem.valid_access_store _ _ _ _ x Hm'_valid).
     destruct Hm' as [m' Hm'].
     exists m'. split.
@@ -5524,7 +5704,7 @@ Proof.
     eapply mem_range_valid. intros. 
     eapply Mem.store_valid_access_1; eauto.
     unfold max_args in *; solve_ptrofs_range.
-Qed.
+Qed. *)
 
  
 
@@ -5577,34 +5757,36 @@ Definition program_gc_inv (p:program) :=
    correct_tinfo p (Int.unsigned finfo_maxalloc) lenv' m'). *)
                                           
 (* deep version of mem_after_asgn  *)
- Inductive rel_mem_asgn {fenv finfo_env p rep_env} args_b args_ofs m L: list L6.cps.val -> list N -> list Values.val -> Prop :=
+ Inductive rel_mem_asgn' {fenv finfo_env p rep_env} args_b args_ofs m L: list L6.cps.val -> list N -> list Values.val -> Prop :=
   | rma_cons: forall  i v6 v7  vs6 inf vs7, 
-    rel_mem_asgn args_b args_ofs  m L vs6 inf vs7 ->
+    rel_mem_asgn' args_b args_ofs  m L vs6 inf vs7 ->
     Mem.loadv int_chunk m (Vptr args_b (Ptrofs.add args_ofs (Ptrofs.repr (int_size * (Z.of_N i))))) = Some v7 ->
     repr_val_L_L6_L7_id fenv finfo_env p rep_env v6 m L v7 ->
-     rel_mem_asgn args_b args_ofs  m L (v6::vs6) (i::inf) (v7::vs7)
+     rel_mem_asgn' args_b args_ofs  m L (v6::vs6) (i::inf) (v7::vs7)
 | rma_nil:
-    rel_mem_asgn args_b args_ofs  m L [] [] []. 
+    rel_mem_asgn' args_b args_ofs  m L [] [] []. 
 
+Definition rel_mem_asgn {fenv finfo_env p rep_env} args_b args_ofs m L vs1 inf vs2 := @rel_mem_asgn' fenv finfo_env p rep_env args_b args_ofs m L (skipn nParam vs1) (skipn nParam inf) (skipn nParam vs2).
+ 
  Theorem rel_mem_asgn_length:
    forall {fenv finfo_env p rep_env m L args_b args_ofs ys inf vs},
      @rel_mem_asgn fenv finfo_env p rep_env args_b args_ofs m L ys inf vs ->
     length ys = length vs.
- Proof.
+ Proof. Admitted. (*
    induction ys; intros.
    inv H; auto.
    inv H. simpl. erewrite IHys. reflexivity.
    eauto.
- Qed.
+ Qed. *)
 
  
  Theorem rel_mem_asgn_nthN:
   forall {L rep_env finfo_env fenv args_b args_ofs p  m vs6 inf vs7 v6 v7 n},
   @rel_mem_asgn fenv finfo_env p rep_env args_b args_ofs  m L vs6 inf vs7 -> 
-  nthN vs6 n = Some v6 ->
-  nthN vs7 n = Some v7 ->
+  nthN (skipn nParam vs6) n = Some v6 ->
+  nthN (skipn nParam vs7) n = Some v7 ->
   repr_val_L_L6_L7_id fenv finfo_env p rep_env v6 m L v7.
-Proof.
+Proof. Admitted. (*
   induction vs6; intros.
   inv H0.
   destruct vs7. inv H1.
@@ -5613,7 +5795,7 @@ Proof.
   apply nthN_pos_pred in H0.
   apply nthN_pos_pred in H1.
   eapply IHvs6; eauto.
-Qed.
+Qed. *)
 
 
  Theorem cons_getlist: forall {A y ys rho vs},
@@ -5631,13 +5813,13 @@ Qed.
    forall fenv finfo_env p rep_env args_b args_ofs m L vs6 locs vs7,
    @rel_mem_asgn fenv finfo_env p rep_env args_b args_ofs  m L vs6 locs vs7 ->
      mem_after_asgn args_b args_ofs m locs vs7.
- Proof.
+ Proof. Admitted. (*
    induction vs6; intros.
    - inv H.
      constructor.
    - inv H.
      constructor; eauto.
- Qed.
+ Qed. *)
  
 Theorem rel_mem_of_asgn: forall fenv finfo_env  rep_env args_b args_ofs p lenv m rho L ys inf vs7 vs6,
  mem_of_asgn_v args_b args_ofs p lenv m ys inf vs7 ->
@@ -5646,7 +5828,7 @@ Theorem rel_mem_of_asgn: forall fenv finfo_env  rep_env args_b args_ofs p lenv m
             exists v6, M.get x rho = Some v6 /\
                        repr_val_id_L_L6_L7_id fenv finfo_env p rep_env v6 m L lenv x) ->
  @rel_mem_asgn fenv finfo_env p rep_env args_b args_ofs m L vs6 inf vs7.
-Proof.
+Proof. Admitted. (*
   induction ys; intros.
   -   inv H0; inv H. constructor.
   - apply cons_getlist in H0. destruct H0 as [v [vs' [Heqvs [Hgar Hgysr]]]]. subst.
@@ -5658,7 +5840,7 @@ Proof.
     rewrite H2 in H5. inv H5. rewrite H in Hgar. inv Hgar. auto.
     rewrite H2 in H5; inv H5. rewrite H2 in H7; inv H7.
     rewrite H5 in H8; inv H8. rewrite H in Hgar. inv Hgar. auto.
-Qed.    
+Qed. *)
 
 (* invariant for GC, needs to be shown to be provable from GC proof *)
 (* OS: Changed returned vs7 into vs7' s.t. the pointers can have changed (but represent the same values in L6) *)
@@ -5825,57 +6007,66 @@ Admitted.
 *)
 
 
+
 Theorem find_symbol_map:
-  forall p map id v, 
-    find_symbol_domain p map ->
-    var_or_funvar id p v (makeVar id v map).
+  forall p fenv id v, 
+    find_symbol_domain p fenv ->
+    var_or_funvar id fenv p v (makeVar id v fenv).
 Proof.
-  intros. unfold makeVar.
-  destruct (cps.M.get v map) eqn:Hgvm.
-  - econstructor. eapply H. eauto.
-  - econstructor.
+  intros. specialize (H v). inv H.
+  destruct (cps.M.get v fenv) eqn:Hgvm.
+  - destruct (H0 (ex_intro _ f (eq_refl _))). econstructor. apply H.
+  - unfold makeVar. rewrite Hgvm. econstructor.
     destruct (Genv.find_symbol (Genv.globalenv p) v) eqn:Hgpv; auto.
     exfalso.
-    specialize (H v). 
-    eapply H in Hgpv. rewrite Hgvm in Hgpv. inv Hgpv.
-    Unshelve. auto. auto.
+    destruct (H1 (ex_intro _ b (eq_refl _))).
+    inv H.
 Qed.
 
-
 Theorem find_symbol_map_f:
-    forall p map id v, 
-    find_symbol_domain p map ->
-    var_or_funvar_f id p v = makeVar id v map.
+    forall p fenv id v, 
+    find_symbol_domain p fenv ->
+    var_or_funvar_f id fenv p v = makeVar id v fenv.
 Proof.
   intros. apply var_or_funvar_of_f.
   apply find_symbol_map; auto.
 Qed.
-  
-Theorem asgnAppVars_correct:
-  forall p map,
-    find_symbol_domain p map ->
-    forall vs ind s,   
-      asgnAppVars' argsIdent threadInfIdent vs ind map = Some s ->
-      repr_asgn_fun'  argsIdent threadInfIdent p vs ind s.
-Proof.
-  intros p map Hmap.
-  induction vs; intros.
-  - destruct ind; inv H. 
-  - destruct ind. inv H.
-    simpl in H. destruct vs. destruct ind.
-    2: inv H.
-    inv H.
-    + (* last one *)
-      erewrite <- find_symbol_map_f; eauto.
-      constructor.
-    +  (* IH *)
-      destruct ( asgnAppVars' argsIdent threadInfIdent (p0 :: vs) ind map) eqn:Happ.
-      2: inv H.
-      apply IHvs in Happ. inv H. 
-      erewrite <- find_symbol_map_f. 2: eauto.
-      constructor. auto.
-Qed.
 
+
+Theorem asgnAppVars_correct:
+  forall p fenv,
+    forall vs avs ind aind s,
+    find_symbol_domain p fenv ->
+      avs = skipn nParam vs ->
+      aind = skipn nParam ind ->
+      asgnAppVars' argsIdent threadInfIdent vs ind fenv = Some s ->
+      repr_asgn_fun' argsIdent threadInfIdent fenv p avs aind s.
+Proof.
+  intros p fenv vs avs. generalize vs. clear vs.
+  induction avs; intros vs ind aind s Hfenv Hvs Hind Hasgn; unfold asgnAppVars' in Hasgn.
+  - destruct aind; rewrite <- Hvs in Hasgn; rewrite <- Hind in Hasgn; inv Hasgn.
+    + constructor.
+  - destruct aind; rewrite <- Hvs in Hasgn; rewrite <- Hind in Hasgn; [ inv Hasgn | ].
+    destruct vs; [inv Hvs | ].
+    destruct ind; [inv Hind | ].
+    symmetry in Hvs.
+    set (Hvs' := skipn_cons nParam p0 a vs avs Hvs).
+    symmetry in Hvs'.
+    symmetry in Hind.
+    set (Hind' := skipn_cons nParam n0 n ind aind Hind).
+    symmetry in Hind'.
+    simpl in Hasgn.
+    destruct (asgnAppVars'' argsIdent threadInfIdent avs aind fenv) eqn:Happ.
+    2: inv Hasgn.
+    specialize (IHavs _ _ _ s0 Hfenv Hvs' Hind').
+    unfold asgnAppVars' in IHavs.
+    rewrite <- Hvs' in IHavs.
+    rewrite <- Hind' in IHavs.
+    apply IHavs in Happ.
+    inv Hasgn.
+    erewrite <- find_symbol_map_f; eauto.
+    exact (repr_asgn_cons _ _ _ _ _ _ _ _ s0 Happ).
+Qed.    
 
 Theorem repr_make_case_switch:
   forall x ls ls',
@@ -5960,11 +6151,11 @@ Proof.
 Qed.
  
 Theorem nth_proj_assign': 
-      forall p map,
-        find_symbol_domain p map ->
+      forall p fenv,
+        find_symbol_domain p fenv ->
         forall v l a n,
-        Forall_statements_in_seq' (is_nth_projection_of_x threadInfIdent p v) 
-                                  (a :: l) (assignConstructorS' threadInfIdent map v n (a :: l)) (Z.of_nat n).
+        Forall_statements_in_seq' (is_nth_projection_of_x threadInfIdent fenv p v) 
+                                  (a :: l) (assignConstructorS' threadInfIdent fenv v n (a :: l)) (Z.of_nat n).
 Proof.
   induction l; intros.
   - (* last *)
@@ -5983,11 +6174,11 @@ Qed.
 
 
 Theorem nth_proj_assign:
-      forall p map,
-        find_symbol_domain p map ->
+      forall p fenv,
+        find_symbol_domain p fenv ->
         forall v l,
           length l > 0 ->
-      Forall_statements_in_seq (is_nth_projection_of_x threadInfIdent p v) l (assignConstructorS' threadInfIdent map v 0 l).
+      Forall_statements_in_seq (is_nth_projection_of_x threadInfIdent fenv p v) l (assignConstructorS' threadInfIdent fenv v 0 l).
 Proof.
   induction l.
   intros Hl. inv Hl.
@@ -5996,12 +6187,12 @@ Proof.
 Qed.
 
 Theorem repr_asgn_constructorS:
-  forall p cenv ienv  rep_env map v c l s name it n,
-      find_symbol_domain p map ->
+  forall p cenv ienv  rep_env fenv v c l s name it n,
+      find_symbol_domain p fenv ->
   correct_crep_of_env cenv  rep_env ->
   M.get c cenv = Some  (name , it, N.of_nat (length l), n) ->
-        assignConstructorS allocIdent threadInfIdent cenv ienv map v c l = Some s -> 
-repr_asgn_constr allocIdent threadInfIdent p rep_env v c l s.
+        assignConstructorS allocIdent threadInfIdent cenv ienv fenv v c l = Some s -> 
+repr_asgn_constr allocIdent threadInfIdent fenv p rep_env v c l s.
 Proof.
   intros p cenv ienv  rep_env map v c l s name it n Hsymbol; intros.
   unfold assignConstructorS in *.
@@ -6068,10 +6259,10 @@ Proof.
   destruct  (n0 =? 0)%N; inv H. auto.
 Qed.  
   
-
+(* Main Theorem *)
 Theorem translate_body_correct:
   forall fenv cenv ienv  p rep_env map,
-    find_symbol_domain p map ->
+    find_symbol_domain p fenv ->
     correct_crep_of_env cenv rep_env ->
     forall  e stm,
       correct_cenv_of_exp cenv e ->
@@ -6082,7 +6273,7 @@ Proof.
   induction e using exp_ind'; intros stm Hcenv; intros.
   - (* Econstr *) 
     simpl in H.
-    destruct (assignConstructorS allocIdent threadInfIdent cenv ienv map v t l) eqn:H_eqAssign.
+    destruct (assignConstructorS allocIdent threadInfIdent cenv ienv fenv v t l) eqn:H_eqAssign.
     destruct (translate_body argsIdent allocIdent limitIdent threadInfIdent tinfIdent isptrIdent caseIdent e fenv cenv ienv map) eqn:H_eqTranslate; inv H.
     2: inv H.
     constructor.
@@ -6155,18 +6346,52 @@ Proof.
       eapply IHe.
       eapply Forall_constructors_subterm. apply Hcenv. constructor. constructor.
       reflexivity.
-  - (* Efun *)
-    inv H.
+  - (* Efun *)  
+    inv H. 
   - (* Eapp *)
-    simpl in H. destruct (cps.M.get t fenv) eqn:Hffenv. 2: inv H.
-    
-    
-    destruct ( asgnAppVars argsIdent threadInfIdent tinfIdent l (snd f) map) eqn:Happvar; inv H.
-    unfold asgnAppVars in *.
-    destruct (asgnAppVars' argsIdent threadInfIdent l (snd f) map) eqn:Happvar'; inv Happvar.
-    erewrite <- find_symbol_map_f. 2: eauto.
+    unfold translate_body in H.
+    destruct (cps.M.get t fenv) eqn:Hffenv. 2:inv H. 
+    destruct f as [n locs].
+    set (avs := skipn nParam l).
+    set (aind := skipn nParam locs).
+    set (bvs := firstn nParam l).
+    assert (vsEq : avs = skipn nParam l). reflexivity.
+    assert (indEq : aind = skipn nParam locs). reflexivity. 
+    assert (bvsEq : bvs = firstn nParam l). reflexivity.
+    unfold asgnAppVars in H. unfold asgnAppVars' in H.
+    simpl (Monad.pbind (Some (n, locs))) in H.
+    assert (H' : Monad.pbind
+           match asgnAppVars'' argsIdent threadInfIdent (skipn nParam l) (skipn nParam locs) fenv with
+           | Some s =>
+               Monad.ret
+                 (Ssequence
+                    (Sset argsIdent
+                       (Efield
+                          (Ederef (Etempvar tinfIdent (Tpointer (Tstruct threadInfIdent noattr) noattr))
+                             (Tstruct threadInfIdent noattr)) argsIdent (Tarray L6_to_Clight.uval maxArgs noattr)))
+                    s)
+           | None => None
+           end
+           (fun asgn : statement =>
+            Monad.ret
+              (Ssequence
+                 (Ssequence
+                    (Ssequence asgn
+                       (Sassign
+                          (Efield
+                             (Ederef (Etempvar tinfIdent (Tpointer (Tstruct threadInfIdent noattr) noattr))
+                                (Tstruct threadInfIdent noattr)) allocIdent valPtr) (Etempvar allocIdent valPtr)))
+                    (Sassign
+                       (Efield
+                          (Ederef (Etempvar tinfIdent (Tpointer (Tstruct threadInfIdent noattr) noattr))
+                             (Tstruct threadInfIdent noattr)) limitIdent valPtr) (Etempvar limitIdent valPtr)))
+                 (mkCall threadInfIdent tinfIdent
+                         (Ecast (makeVar threadInfIdent v fenv) (mkFunTy threadInfIdent (length (firstn nParam l)))) l))) = Some stm). apply H. clear H.
+    rewrite <- vsEq in H'. rewrite <- indEq in H'. rewrite <- bvsEq in H'. simpl in H'.
+    destruct (asgnAppVars'' argsIdent threadInfIdent avs aind fenv) eqn:Happvar; inv H'.
+    erewrite <- find_symbol_map_f. 2: eauto. 
     econstructor.
-    eauto. constructor.
+    eauto. eauto. eauto. constructor.
     eapply asgnAppVars_correct; eauto.    
   - (* Eprim *)
     inv H. 
@@ -6197,8 +6422,9 @@ Inductive proper_cTyInfo: cTyInfo -> Prop :=
  
 (* cenv is proper if cTyInfo is proper, and that there is a unique (ty, ord) pair for each constructors  *)
 
+
 Definition proper_cenv (cenv:cEnv):=
-  forall {c name it a ord},
+  forall c name it a ord,
     M.get c cenv = Some (name, it, a, ord) ->
     proper_cTyInfo (name, it, a, ord) /\
       ~ (exists c' name' a', c <> c' /\
@@ -6521,6 +6747,7 @@ Qed.
 Ltac unsigned_ptrofs_range :=
   split; [apply Ptrofs.unsigned_range |  etransitivity;  [apply Ptrofs.unsigned_range_2 | rewrite ptrofs_mu; archi_red; reflexivity] ].
 
+(* Main Theorem *)
 Theorem repr_bs_L6_L7_related:
   forall p rep_env cenv fenv finfo_env ienv,
     program_inv p ->
@@ -6683,7 +6910,7 @@ Proof.
         
         (* 2 -> use mem_of_Forall_nth_projection to step through the assignment of vs *)
         assert (Hstep_m3 := mem_of_Forall_nth_projection_cast).
-        specialize (Hstep_m3 threadInfIdent p x
+        specialize (Hstep_m3 threadInfIdent fenv p x
                              (Maps.PTree.set allocIdent
                                              (Vptr alloc_b
                                                    (Ptrofs.add alloc_ofs (Ptrofs.mul (Ptrofs.repr (sizeof (globalenv p) val)) (Ptrofs.repr (Z.of_N (a + 1))))))
@@ -6701,7 +6928,8 @@ Proof.
                   (Maps.PTree.set x
                      (Vptr alloc_b (Ptrofs.add alloc_ofs (Ptrofs.mul (Ptrofs.repr (sizeof (globalenv p) val)) (Ptrofs.repr Z.one)))) lenv)) =
              Some (Vptr alloc_b (Ptrofs.add alloc_ofs (Ptrofs.mul (Ptrofs.repr (sizeof (globalenv p) val)) (Ptrofs.repr Z.one))))).
-        rewrite M.gso. rewrite M.gss. reflexivity. intro; apply Hx_not. rewrite H4.  inList. 
+        rewrite M.gso. rewrite M.gss. reflexivity. intro; apply Hx_not. rewrite H4.  inList.
+        (* BROKEN : needs find_symbol_domain p fenv *)
         specialize (Hstep_m3 Htemp ys s0 0%Z m2 (Kseq s' k)). clear Htemp.
         assert (Htemp : (0 <= 0)%Z /\ (0 + Z.of_nat (length ys) <= Ptrofs.max_unsigned)%Z ).
         {
@@ -6831,7 +7059,7 @@ Proof.
             
             inv Hrel_m.  destruct H4.
             eapply exists_getvar_or_funvar_list.
-            Focus 2. eauto.
+            2:{  eauto. }
             intros.
             apply H5. constructor. auto.
           } 
@@ -7090,7 +7318,7 @@ Proof.
                 split. chunk_red; omega.
                 rewrite <- Z.le_add_le_sub_l in H12.    
                 etransitivity. etransitivity.
-                Focus 2. apply H12.
+                2: apply H12.
                 rewrite Nat2Z.inj_succ.
                 rewrite Z.mul_succ_r.
                 assert (0 <= Ptrofs.unsigned alloc_ofs)%Z by apply Ptrofs.unsigned_range.                
@@ -7176,7 +7404,7 @@ Proof.
           - intros. destruct (var_dec x0 x).
                  + (* x0 = x *)
                    subst. split.
-                   Focus 2.
+                   2:{ 
                      intros. rewrite M.gss in H4. inv H4.
                      apply subval_or_eq_fun in H5. destruct H5. destruct H4.
                      assert (Hy0x0 := getlist_In_val _ _ _ _ H H5).
@@ -7187,9 +7415,8 @@ Proof.
                      destruct Hrel_mL' as [Hrel_mL' [Hrel_closed Hrel_f]]. split.
                      eapply repr_val_id_L_sub_locProp.
                      eapply repr_val_id_L_unchanged.                     
-                     Focus 2. eauto.
-                     Focus 2. 
-                     intro. intro. intro. apply bind_n_after_ptr_def. left; auto.
+                     2: eauto.
+                     2:{ intro. intro. intro. apply bind_n_after_ptr_def. left; auto. }
                      apply repr_val_id_set. apply repr_val_id_set.
                      auto.
                      (* unique binding env should take care of this one? ...also since function not bound, but Hrel_mL'...*)
@@ -7217,7 +7444,7 @@ Proof.
                      eapply correct_fundefs_unchanged_global with (m := m).
                      apply Hrel_f.
                      auto.
-                     auto.
+                     auto. }
                      
                    intros. eexists. split.
                    rewrite M.gss. reflexivity.
@@ -7312,7 +7539,7 @@ Proof.
 
                     
                   rewrite repr_val_ptr_list_Z.
-                  Focus 2.
+                  2:{ 
                   rewrite H_alloc4. 
                     unfold int_size in *; simpl size_chunk in *.
                     inv Hc_alloc.
@@ -7351,7 +7578,7 @@ Proof.
                     apply Z.add_le_mono; [ | omega];
                     apply Z.add_le_mono; [ | omega];
                     rewrite <- Z.add_0_l at 1;
-                    apply Z.add_le_mono_r; chunk_red; omega.
+                    apply Z.add_le_mono_r; chunk_red; omega. }
                     
                     (* done *)
 
@@ -7418,7 +7645,7 @@ Proof.
                   assert (Hll' := bind_n_after_ptr_exists  (length vs2) alloc_b (Ptrofs.unsigned alloc_ofs + int_size + int_size * Z.of_nat (length vs1)) L). 
                   destruct Hll' as [L' [H_ll' H_eql']].
                   eapply  repr_val_ptr_list_L_Z_sub_locProp with (L := L'); auto.
-                  Focus 2.                  
+                  2:{                   
                   intro. intro. intro. apply bind_n_after_ptr_def.
                   rewrite <- H_eql' in H6.
                   apply bind_n_after_ptr_def in H6.
@@ -7428,7 +7655,7 @@ Proof.
                   rewrite N2Z.inj_add.
                   replace (Z.of_N a) with (Z.of_nat (length ys)) by omega.
                   replace (length ys) with (length vs2). int_red. simpl in H8. simpl Z.of_N. chunk_red; omega.
-                  apply Forall2_length' in Hvs7. auto.
+                  apply Forall2_length' in Hvs7. auto. }
 
                   (* current locprop, from L + 1 to L + 1 + length vs *)
                   assert (H_ll'':= bind_n_after_ptr_exists' (length vs1) alloc_b  (Ptrofs.unsigned alloc_ofs + int_size) L).
@@ -7474,11 +7701,11 @@ Proof.
                   
                   rewrite get_var_or_funvar_list_correct in Hvs7. rewrite <- get_var_or_funvar_list_set in Hvs7.
                   rewrite <- get_var_or_funvar_list_set in Hvs7.
-                  Focus 2. intro.
+                  2:{  intro.
                   assert (Hxrho := getlist_In _ _ _ _ H H6).
                   destruct Hxrho as [vv Hxrho].
-                  eapply Hrho_id; eauto.
-                  Focus 2. intro.
+                  eapply Hrho_id; eauto. }
+                  2:{  intro.
                   inv Hp_id.
                   
                   eapply getlist_In in H; eauto. 
@@ -7486,7 +7713,7 @@ Proof.
                   eapply H8. apply H.
                   right. 
                   left. reflexivity.
-                  left. reflexivity.
+                  left. reflexivity. }
                   rewrite <- get_var_or_funvar_list_correct in Hvs7. 
                     
                   clear Hrel_mL.
@@ -7530,8 +7757,8 @@ Proof.
                     inv H8. rewrite H9 in H1; inv H1.
                     - (* fun *)
                       eapply repr_val_L_sub_locProp.
-                      Focus 2. intro.  intros. eapply bind_n_after_ptr_from_rev in H_ll'. rewrite <- H_ll'.
-                      apply bind_n_after_ptr_def. left. apply H1.
+                      2:{  intro.  intros. eapply bind_n_after_ptr_from_rev in H_ll'. rewrite <- H_ll'.
+                      apply bind_n_after_ptr_def. left. apply H1. }
                       eapply repr_val_L_unchanged; eauto.
                     - (* constr *)
                       rewrite load_ptr_or_int.
@@ -7539,8 +7766,8 @@ Proof.
                       rewrite H9 in H1; inv H1.
                     - 
                       eapply repr_val_L_sub_locProp.
-                      Focus 2. intro.  intros. eapply bind_n_after_ptr_from_rev in H_ll'. rewrite <- H_ll'.
-                      apply bind_n_after_ptr_def. left. apply H1.
+                      2:{ intro.  intros. eapply bind_n_after_ptr_from_rev in H_ll'. rewrite <- H_ll'.
+                      apply bind_n_after_ptr_def. left. apply H1. }
                       eapply repr_val_L_unchanged; eauto.
                       rewrite load_ptr_or_int by auto.
                       inv H8. rewrite H1 in H9. inv H9.                      
@@ -7694,7 +7921,7 @@ Forall2
           destruct Hstep_m3.          
           eapply correct_tinfo_after_nstore.
           
-          Focus 2. eauto.
+          2: eauto.
           
           eapply correct_tinfo_after_store; eauto.
           inv Hc_alloc.
@@ -7707,7 +7934,7 @@ Forall2
           {
             inv Hp_id.
             intro; subst; eapply H5.
-            Focus 2. constructor.
+            2: constructor.
             inList.
           }
           (* alloc is moved to an OK location *)
@@ -7950,7 +8177,7 @@ Forall2
             { inv Hp_id.
               intro; subst.
               eapply H5.
-              Focus 2. constructor.
+              2: constructor.
               inList.
             }
             intro.
@@ -7982,12 +8209,12 @@ Forall2
           destruct Hrepr_m as [Hrepr_m Hrepr_m'].
           destruct (var_dec x0 x).
           * subst.
-            split. Focus 2. 
-              intros. rewrite M.gss in H2. inv H2.
+            split. 
+              2:{ intros. rewrite M.gss in H2. inv H2.
               apply subval_or_eq_fun in H3. destruct H3. destruct H2.
               assert (Hy0x0 := getlist_In_val _ _ _ _ H H3).
               destruct Hy0x0 as [y0 [Hy0 Hy0']].
-              inv Hy0.
+              inv Hy0. }
             
               
             intro. 
@@ -8013,7 +8240,7 @@ Forall2
             intros. rewrite M.gso in H2 by auto.
             eapply Hrepr_m' in H2; eauto.
             destruct H2 as [H2 Hrepr_f].
-            split. Focus 2. auto.
+            split. 2: auto.
             apply repr_val_id_set; auto.
             intro; subst.
             inv Hf_id.
@@ -8036,7 +8263,7 @@ Forall2
           { inv Hp_id.
             intro; subst.
             eapply H3.
-            Focus 2. constructor.
+            2: constructor.
             inList.
           }
 
@@ -8054,9 +8281,9 @@ Forall2
       eauto.
       - inv Hc_env.
         destructAll.
-        apply Forall_constructors_in_constr in H2. destruct (M.get t cenv) eqn:Mtcenv. Focus 2. inv H2. destruct c0. destruct p. destruct p0. destruct p.
+        apply Forall_constructors_in_constr in H2. destruct (M.get t cenv) eqn:Mtcenv. 2: inv H2. destruct c0. destruct p. destruct p0. destruct p.
         econstructor; eauto.        
-        Focus 2. apply getlist_length_eq in H. subst. auto.
+        2:{ apply getlist_length_eq in H. subst. auto. }
         apply Forall_forall. intros.
         assert (Hgiv := getlist_In_val _ _ _ _ H H4).
         destruct Hgiv. destruct H5.
@@ -8253,7 +8480,7 @@ Forall2
             apply nthN_In in H0.
             specialize (Hmem y). destruct Hmem as [Hmem Hmem'].
             specialize (Hmem' _ _ _ _ Hyv6 (subval_or_eq_constr _ _ _ _ H3 H0)). 
-            destruct Hmem' as [Hmem' Hmem_f]. split. Focus 2. auto.
+            destruct Hmem' as [Hmem' Hmem_f]. split. 2: auto.
             apply repr_val_id_set. auto.
             intro. subst.
             inv Hf_id.
@@ -8275,7 +8502,7 @@ Forall2
             rewrite M.gso; auto.
           * intros. specialize (Hmem' _ _ _ _ H2 H3).
             destruct Hmem' as [Hmem' Hmem_f].
-            split. Focus 2. auto.
+            split. 2: auto.
             apply repr_val_id_set. auto.
             inv Hmem'. intro.  inv Hf_id. specialize (H10 x).
             assert ( bound_var (Eproj x t n y e) x) by constructor. apply H10 in H9. 
@@ -8292,7 +8519,7 @@ Forall2
     {
       inv Hp_id.
       intro. eapply H10.
-      Focus 2. subst. constructor.
+      2:{ subst. constructor. }
       inList.
     }
     specialize (IHHev H2 H3 H9).
@@ -8529,14 +8756,14 @@ Forall2
         destruct Hmem_rel' as [Hmem_rel' Hmem_f].
         split. 2: auto.
         apply repr_val_id_set. auto.
-        intro. inv Hp_id. eapply H22. apply H19. Focus 2. right.
+        intro. inv Hp_id. eapply H22. apply H19. 2:{ right.
         eapply bound_var_subval; eauto.
         inv Hmem_rel'.
         inv H31.
         constructor.
         apply name_in_fundefs_bound_var_fundefs.
         eapply find_def_name_in_fundefs. eauto.
-        inv H25. rewrite H32 in H21. inv H21.
+        inv H25. rewrite H32 in H21. inv H21. }
         inList.
         
     }
@@ -8590,7 +8817,7 @@ Forall2
     rewrite M.gso; auto.
     assert (H_dj := disjointIdent). inv H_dj.
     intro; apply H3; subst; inList.    
-  - (* Eapp  *)
+  - (* Eapp  *)  (* CHANGE THIS *)
 
     (* need assumption that unique_binding_env -> done! and functions_not_bound is preserved by all closures (rho', e) in rho - DONE *)
     (* Show protected_id_not_bound_id is preserved by prefixes - done *)
@@ -8910,7 +9137,7 @@ Forall2
       solve_nodup.
       eauto.
       solve_nodup.      
-    }
+    } 
     assert (Hm5 : exists m5 lenv_new',
                 clos_trans state (traceless_step2 (globalenv p))
                            (State F
@@ -9142,11 +9369,11 @@ Forall2
              
             rewrite Ptrofs.signed_repr with (z := int_size%Z) in H12.
             rewrite Ptrofs.signed_repr in H12.
-            Focus 2. split.
+            2:{ split.
             rewrite <- Z.le_add_le_sub_l. etransitivity. 2: eauto.
             unfold Ptrofs.min_signed.  
             inv Hc_alloc.    unfold Ptrofs.half_modulus. unfold Ptrofs.modulus. simpl. unfold Ptrofs.wordsize. unfold Wordsize_Ptrofs.wordsize. chunk_red; archi_red; simpl; omega. 
-            etransitivity; eauto. unfold gc_size; unfold Ptrofs.max_signed. unfold Ptrofs.half_modulus. unfold Ptrofs.modulus.  unfold Ptrofs.wordsize. unfold Wordsize_Ptrofs.wordsize. chunk_red; archi_red; simpl; omega.  
+            etransitivity; eauto. unfold gc_size; unfold Ptrofs.max_signed. unfold Ptrofs.half_modulus. unfold Ptrofs.modulus.  unfold Ptrofs.wordsize. unfold Wordsize_Ptrofs.wordsize. chunk_red; archi_red; simpl; omega. } 
             2:unfold Ptrofs.min_signed; unfold Ptrofs.max_signed; unfold Ptrofs.half_modulus;  unfold Ptrofs.modulus;  unfold Ptrofs.wordsize; unfold Wordsize_Ptrofs.wordsize; chunk_red; archi_red; simpl; omega. 
             rewrite Ptrofs.unsigned_repr in H12. 
             rewrite Ptrofs.unsigned_repr in H12.
@@ -10018,7 +10245,7 @@ solve_nodup. solve_nodup.
         rewrite Ptrofs.mul_one in Hm2.
         eapply Mem.load_store_same in Hm2. simpl in Hm2. destruct v7; inv H3; auto.
         rewrite H in Hxrho. inv Hxrho.
-        eapply repr_val_L_unchanged; eauto.       
+        eapply repr_val_L_unchanged; eauto.        
             Qed.
 
 
