theories/Runtime/mkas.sh
@@ -1,5 +1,6 @@
 #!/bin/sh
-clang -w -S -O2 -fomit-frame-pointer $1.ll
+sh mkllvm.sh $1
+clang -w -S -O2 -fomit-frame-pointer $1.c
 clang -w -S -O2 -fomit-frame-pointer $1CC.ll
-rm $1.ll
+ccomp -w -S -O2 $1.c -o $1ccomp.s
 rm $1CC.ll
