theories/Runtime/mkexec.sh
@@ -1,7 +1,12 @@
 #!/bin/sh
 sh mkllvm.sh $1
-clang -w -O2 -fomit-frame-pointer main.c gc.c $1.c -o $1c.out
-clang -w -O2 -fomit-frame-pointer main.c gc.c $1.ll -o $1.out
+clang -w -O2 -fomit-frame-pointer main.c gc.c $1.c -o $1.out
 clang -w -O2 -fomit-frame-pointer main.c gc.c $1CC.ll -o $1CC.out
-rm $1.ll
+clang -w -O2 main.c gc.c $1.c -o $1Frame.out
+clang -w -O2 main.c gc.c $1CC.ll -o $1CCFrame.out
+ccomp -w -O2 main.c gc.c $1.c -o $1ccomp.out
+if [ "$2" = '-make-ocaml' ]; then
+    ocamlbuild $1.native
+    ocamlbuild $1.byte
+fi
 rm $1CC.ll
